Core/LinFacts.v
@@ -1,0 +1,14 @@
+From LHL.Core Require Import
+    Program
+    Specs
+    Traces
+    Linearizability.
+
+Theorem lin_obs_ref {E F} : 
+    forall (spec' spec : Spec E) (impl : Impl E F) ,
+        Lin spec' spec -> 
+        layerRefines (mkLayer spec' impl) (mkLayer spec impl).
+Proof.
+    intros. intro. intro.
+    unfold IsTraceOfSpec.
+    destruct H0. destruct H0.
