Core/Linearizability.v
@@ -10,3 +10,7 @@ Definition KConc {E} (spec : Spec E) : Spec E := overObj (idLayer spec).
 
 Definition Lin {E} (spec' : Spec E) (spec : Spec E) :=
     specRefines spec' (KConc spec).
+
+
+
+
