Core/ProgramFacts.v
@@ -1,0 +1,16 @@
+From LHL Require Import
+    Program.
+
+Definition frobProgram {E Ret} (p : Prog E Ret) :
+  Prog E Ret :=
+  match p with
+    | Bind e f => Bind e f
+    | Return a => Return a
+    | NoOp p' => NoOp p'
+  end.
+
+Theorem frobProgId {E Ret} (p : Prog E Ret) :
+  p = frobProgram p.
+Proof.
+  destruct p; reflexivity.
+Defined.
