Core/VCompFacts.v
@@ -1,0 +1,67 @@
+ From Paco Require Import paco.
+
+From LHL.Core Require Import
+  Program
+  Specs
+  Traces
+  Eutt
+  ProgramFacts.
+From LHL.Util Require Import
+  Util.
+
+Lemma substIdImpl_is_id_l {M R} (p : Prog M R)
+  : eutt ieq (substProg idImpl p) p.
+Proof.
+  enough (J : forall q p : Prog M R,
+             (q = substProg (fun _ m => Bind m Return) p \/
+              q = NoOp (substProg (fun _ m => Bind m Return) p)) ->
+             eutt ieq q p).
+  { apply J. left; reflexivity. }
+  clear. pcofix SELF. intros q p.
+  enough (J : paco2 (euttF ieq) r (substProg (fun _ m => Bind m Return) p) p).
+  { intros []; subst; [ apply J | apply euttF_Noop_L, J ]. }
+  pfold.
+  destruct p.
+  - rewrite (frobProgId (substProg _ _)). cbn. constructor.
+    rewrite (frobProgId (bindSubstProg _ _ _)). cbn.
+    constructor; [ constructor | ].
+    intros x. right.
+    rewrite (frobProgId (bindSubstProg _ _ _)). cbn.
+    apply SELF. right. reflexivity.
+  - rewrite (frobProgId (substProg _ _)). cbn. constructor.
+  - rewrite (frobProgId (substProg _ _)). cbn. constructor.
+    right. apply SELF. left. reflexivity.
+Defined.
+
+Lemma substIdImpl_is_id_r {E F} (impl : Impl E F)
+  {R} (f : F R)
+  : eutt ieq (substProg impl (idProg f)) (impl _ f).
+Proof.
+  rewrite (frobProgId (substProg _ _)). cbn.
+  apply eutt_NoOp_l.
+  remember (impl R f) as p eqn:E0. clear E0 f.
+  revert p. pcofix SELF. intros p.
+  pfold.
+  destruct p;
+    rewrite (frobProgId (bindSubstProg _ _ _)); cbn; constructor.
+  - constructor.
+  - right; auto.
+  - rewrite (frobProgId (substProg _ _)); cbn; constructor.
+  - right; auto.
+Qed.
+
+Theorem idImpl_is_identity_l {E F Ret} : 
+    forall (impl : Impl E F) , 
+    euttImpl (Ret := Ret) ieq (idImpl |> impl) impl.
+Proof.
+  intros. unfold euttImpl. intros.
+  apply substIdImpl_is_id_l.
+Qed.
+
+Theorem idImpl_is_identity_r {E F Ret} : 
+    forall (impl : Impl E F) , 
+    euttImpl (Ret := Ret) ieq (impl |> idImpl) impl.
+Proof.
+  intros. unfold euttImpl. intros.
+  apply substIdImpl_is_id_r.
+Qed.
