Util/Tactics.v
@@ -1,0 +1,12 @@
+From Coq Require Import Eqdep.
+
+Ltac injpair_ :=
+  repeat
+    lazymatch goal with
+    | [ H : existT ?P ?R _ = existT ?P ?R _ |- _ ] => apply inj_pair2 in H
+    end.
+
+Ltac injpair :=
+  subst; injpair_; subst.
+
+Ltac inv H := inversion H; clear H; subst.
