Util/Util.v
@@ -1,0 +1,4 @@
+Notation IRel M N := (forall X, M X -> N X -> Prop) (only parsing).
+
+Definition ieq {M : Type -> Type} R (e1 e2 : M R) : Prop := e1 = e2.
+Hint Unfold ieq : core.
